# Exercise 4.7ab

## Problem

A variable with PMF

$$
p(k) = \binom{k + r - 1}{k} (1 - p)^r p^k
$$

is a negative binomial random variable with support in non-negative integers.
It has two parameters $r > 0$ and $p \in (0, 1)$. We denote

$$
X|r,p \sim \text{NB}(r, p).
$$

a) Let us reparameterize the negative binomial distribution with $q = 1 - p$.
   Find the PMF of $X \sim \text{NB}(1, q)$. Do you recognize this distribution?

b) Show that the sum of two negative binomial random variables with the same
   $p$ is also a negative binomial random variable.

## Solution

a) $X \sim \text{NB}(1, q)$

$$
p_X(k) = \binom{k + r - 1}{k} (1 - p)^r p^k =
    \binom{k + 1 - 1}{k} q^1 (1 - q)^k = (1 - q)^k q .
$$

This is PMF of a geometric random variable with parameter $q$.

b) Let $X \sim \text{NB}(r_X, p)$ and $Y \sim \text{NB}(r_Y, p)$.

$$
\begin{aligned}
    p_{X+Y}(k) &= P(X + Y = k) = \sum_{y = 0}^\infty P(X = k - y) P(Y = y) =
        \sum_{y = 0}^k p_X(k - y) p_Y(y) = \\
    &= \sum_{y = 0}^k \binom{k - y + r_X - 1}{k - y} (1 - p)^{r_X} p^{k - y}
        \cdot \binom{y + r_Y - 1}{y} (1 - p)^{r_Y} p^y.
\end{aligned}
$$

Sum only needs to go to $k$, since support of negative binomial distribution
does not contain negative numbers $k - y$. Now we can see that summing all
possible products of binomials for choosing $k - y$ elements out of $r_X$ and
$y$ out of $p_Y$ with replacement is the same as choosing $k$ elements
out of $p_X + p_Y$:

$$
p_{X+Y}(k) = \binom{k + r_X + r_Y - 1}{k} (1 - p)^{r_X + r_Y} p^k,
$$

thus

$$
X + Y \sim \text{NB}(r_X + r_Y, p).
$$
