# Exercise 7.6

## Problem

Let $X \sim \text{Beta}(\alpha, \beta)$.

a) Find $\mathbb{E}[X]$.

b) Find $Var[X]$.

## Solution

PDF of beta distribution is

$$
f_X(x) = \frac{x^{\alpha - 1} (1 - x)^{\beta - 1}}{B(\alpha, \beta)}
$$

for $x \in [0, 1]$ and beta function is defined as

$$
B(x, y) = \int_0^1 t^{x-1} (1 - t)^{y-1}\ dt .
$$

a) We start calculating expected value from the definition:

$$
\mathbb{E}[X] = \int_0^1 x f_X(x)\ dx =
\int_0^1 x \frac{x^{\alpha - 1} (1 - x)^{\beta - 1}}{B(\alpha, \beta)}\ dx =
\frac{1}{B(\alpha, \beta)} \int_0^1 x^\alpha (1 - x)^{\beta - 1}\ dx =
\frac{B(\alpha + 1, \beta)}{B(\alpha, \beta)}.
$$

Now we use $B(x + 1, y) = B(x, y) \frac{x}{x + y}$ and get

$$
\mathbb{E}[X] = \frac{B(\alpha + 1, \beta)}{B(\alpha, \beta)} =
\frac{B(\alpha, \beta) \alpha}{B(\alpha, \beta) (\alpha + \beta)} =
\frac{\alpha}{\alpha + \beta} .
$$

b) For variance we first need second moment:

$$
\begin{aligned}
\mathbb{E}[X^2] &= \int_0^1 x^2 f_X(x)\ dx =
\int_0^1 x^2 \frac{x^{\alpha - 1} (1 - x)^{\beta - 1}}{B(\alpha, \beta)}\ dx =
\frac{1}{B(\alpha, \beta)} \int_0^1 x^{\alpha + 1} (1 - x)^{\beta - 1}\ dx =
\frac{B(\alpha + 2, \beta)}{B(\alpha, \beta)} = \\
&= \frac{B(\alpha + 1, \beta) (\alpha + 1)}{B(\alpha, \beta) (\alpha + \beta + 1)} =
\frac{B(\alpha, \beta) \alpha (\alpha + 1)}{
    B(\alpha, \beta) (\alpha + \beta) (\alpha + 1 + \beta)
} = \frac{\alpha (\alpha + 1)}{(\alpha + \beta) (\alpha + \beta + 1)} .
\end{aligned}
$$

Now compute variance from definition:

$$
\begin{aligned}
Var[X] &= \mathbb{E}[X^2] - \mathbb{E}[X]^2 =
\frac{\alpha (\alpha + 1)}{(\alpha + \beta) (\alpha + \beta + 1)} -
\left(\frac{\alpha}{\alpha + \beta}\right)^2 = \\
&= \frac{\alpha (\alpha + 1) (\alpha + \beta) - \alpha^2 (\alpha + \beta + 1)}{
    (\alpha + \beta)^2 (\alpha + \beta + 1)
} = \frac{\alpha^3 + \alpha^2 + \alpha^2\beta + \alpha\beta - \alpha^3 -
    \alpha^2 - \alpha^2\beta}{(\alpha + \beta)^2 (\alpha + \beta + 1)} \\
&= \frac{\alpha \beta}{(\alpha + \beta)^2 (\alpha + \beta + 1)} .
\end{aligned}
$$
